Operations.dfy
@@ -1,0 +1,121 @@
+include "Type.dfy"
+include "Property.dfy"
+module Operations {
+  import opened Type
+  import opened Property
+
+  // This is the pre-condition for rotate_left
+  predicate right_leaning_red_link(t: Rb_tree)
+  {
+    match t
+    case Node(_, _, Null, Node(Red, _, _, _)) => true
+    case Node(_, _, Node(Black, _, _, _), Node(Red, _, _, _)) => true
+    case _ => false
+  }
+
+  function rotate_left(h: Rb_tree): Rb_tree
+    requires right_leaning_red_link(h)
+    ensures !right_leaning_red_link(rotate_left(h))
+    decreases h
+  {
+    match h
+    case Node(h_color, h_key, h_left, h_right) =>
+      match h_right
+      case Node(Red, x_key, x_left, x_right) =>
+        var new_h := Node(Red, h_key, h_left, x_left);
+        var new_x := Node(h_color, x_key, new_h, x_right);
+        new_x
+  }
+
+
+  // This is the pre-condition for rotate_right
+  predicate double_left_red_link(h: Rb_tree)
+  {
+    match h
+    case Node(h_color, h_key, Node(Red, x_key, Node(Red, _, _, _), _), _) => true
+    case _ => false
+  }
+
+  function rotate_right(h: Rb_tree): Rb_tree
+    requires h.Node?
+    requires double_left_red_link(h)
+    // requires !right_leaning_red_link(h) true but the proof uhhhh
+    requires h.color == Black
+    ensures !double_left_red_link(rotate_right(h))
+    decreases h
+  {
+    match h
+    case Node(h_color, h_key, Node(Red, x_key, Node(Red, ll_key, ll_left, ll_right), x_right), h_right) =>
+      var new_h := Node(Red, h_key, x_right, h_right);
+      var new_x := Node(h_color, x_key, Node(Red, ll_key, ll_left, ll_right), new_h);
+      assert new_x.color == h_color;
+      new_x
+  }
+
+
+  // this is the precondition for color flip
+  predicate hasRedChildren(h: Rb_tree)
+  {
+    match h
+    // I think we might need to help dafny to prove that this node is black
+    case Node(Black, _, Node(Red, _, _, _), Node(Red, _, _, _)) => true
+    case _ => false
+  }
+
+  function flip_color(h: Rb_tree): Rb_tree
+    requires hasRedChildren(h)
+    ensures !hasRedChildren(flip_color(h))
+    decreases h
+  {
+    match h
+    case Node(_, key, Node(_, l_key, l_left, l_right), Node(_, r_key, r_left, r_right)) =>
+      var new_left := Node(Black, l_key, l_left, l_right);
+      var new_right := Node(Black, r_key, r_left, r_right);
+      var new_h := Node(Red, key, new_left, new_right);
+      new_h
+  }
+
+  function nodeColor(t: Rb_tree): Color
+  {
+    match t
+    case Null => Black
+    case Node(c, _, _, _) => c
+  }
+
+  function insert_recur(t: Rb_tree, key: int): Rb_tree
+    decreases t
+  {
+    var inserted := match t
+      case Null => Node(Red, key, Null, Null)
+      case Node(color, k, left, right) =>
+        if key < k then Node(color, k, insert_recur(left, key), right)
+        else if key > k then Node(color, k, left, insert_recur(right, key))
+        else Node(color, k, left, right);
+
+    var step1 := if nodeColor(inserted.right) == Red && nodeColor(inserted.left) == Black
+                 then rotate_left(inserted)
+                 else inserted;
+
+    var step2 := match step1
+      case Node(_, _, Node(Red, _, Node(Red, _, _, _), _), _) => rotate_right(step1)
+      case _ => step1;
+
+    var step3 := match step2
+      case Node(Black, _, Node(Red, _, _, _), Node(Red, _, _, _)) => flip_color(step2)
+      case _ => step2;
+
+    step3
+  }
+  // Wrapper function for the recursive and then change root color
+  function insert(t: Rb_tree, key: int): Rb_tree
+    requires rb_tree_property_2(t)
+    ensures rb_tree_property_2(insert(t, key))
+  {
+    var new_tree := insert_recur(t, key);
+
+    //Ensure the root is always Black from the side effect of flipcolor
+    match new_tree
+    case Null => Null
+    case Node(_, k, l, r) => Node(Black, k, l, r)
+  }
+}
